Let $\eta$ be a node that satisfies the pre-regularization and regularization unifiability properties, and suppose to the contrary that it does not satisfy  the post-deletion unifiability property. 
Let $p\in \mathcal{S}(\eta)$ be a safe literal of $\eta$ such that for some node $\eta'$, there exists a literal $\ell' \in \eta'$ such that $(p,\ell')$ are unifiable in $\psi$ but not in $\psi\setminus\{\eta\}$, i.e. $(p^\dagger,\ell'^\dagger)$ is not unifiable. Let $\sigma_0$ be a most general unifier of $(p,\ell')$ in $\psi$ (note that $\sigma_0$ exists since $\eta$ satisfies the pre-regularization property), and let $\sigma_1,\ldots,\sigma_n$ be the unifiers applied to $p$ in $\psi$ between $\eta$ and $\eta'$, so that in $\psi$, $p=\sigma_n\sigma_{n-1}\ldots\sigma_1\sigma_0\dual{\ell'}$. Since $\eta$ satisfies the regularization property, if $\eta_1$ is the parent to replace $\eta$, we must have $\sigma\eta_1\subseteq \phi = \mathcal{S}(\eta)$, and in particular, $\sigma p_1 = p = \sigma_n\ldots\sigma_1\sigma_0\dual{\ell'}$ for some $p_1\in \eta_1$. 
%Thus there is some subset $\mathcal{I}\subseteq [1,n]$ such that $\sigma p_1 = \sigma_m'\ldots\sigma_1'\dual{\ell'}$ since FO-delete uses the same unifiers. 
Note that $p^\dagger = \sigma_p p = \sigma_p\sigma_n\ldots\sigma_1\sigma_0\dual{\ell'}$ (where the first equality holds since $p^\dagger$ corresponds to $p$, and thus the two literals are unifiable) but also that $\dual{\ell'} = \sigma_\ell\ell'$ for some $\sigma_\ell$ (by definition as $\ell$ as a pivot). So now we have $p^\dagger =  \sigma_p\sigma_n\ldots\sigma_1\sigma_0\sigma_\ell\ell'$, so letting $\sigma''=\sigma_p\sigma_m'\ldots\sigma_1'\sigma_\ell$ we have that $p^\dagger = \sigma'' \ell$, i.e. that $(p^\dagger,\ell^\dagger)$ are unifiable via $\sigma''$, a contradiction.
%Note that $p^\dagger =  \sigma_m'\ldots\sigma_1'\dual{\ell'}$ but also that $\dual{\ell'} = \sigma_\ell\ell'$ for some $\sigma_\ell$ (by definition as $\ell$ as a pivot). So now we have $p^\dagger =  \sigma_m'\ldots\sigma_1'\sigma''\ell$, so letting $\sigma''=\sigma_m'\ldots\sigma_1'\sigma_\ell$ we have that $p^\dagger = \sigma'' \ell$, i.e. that $(p^\dagger,\ell^\dagger)$ are unifiable via $\sigma''$, a contradiction.





%newer, but still old
Let $\eta$ be a node that satisfies the pre-regularization and regularization unifiability properties.
Let $p\in \mathcal{S}(\eta)$ be a safe literal of $\eta$ such that for some node $\eta'$, there exists a literal $\ell' \in \eta'$ such that $(p,\ell')$ are unifiable in $\psi$. We will show that $(p^\dagger,\ell'^\dagger)$ is unifiable in $\psi\setminus\{\eta\}$. 
Let $\sigma_0$ be a most general unifier of $(p,\ell')$ in $\psi$ (note that $\sigma_0$ exists since $\eta$ satisfies the pre-regularization property), and let $\sigma_1,\ldots,\sigma_n$ be the unifiers applied to $p$ in $\psi$ between $\eta$ and $\eta'$, so that in $\psi$, $p=\sigma_n\sigma_{n-1}\ldots\sigma_1\sigma_0\dual{\ell'}$. Since $\eta$ satisfies the regularization property, if $\eta_1$ is the parent to replace $\eta$, we must have $\sigma\eta_1\subseteq \phi = \mathcal{S}(\eta)$, and in particular, $\sigma p_1 = p = \sigma_n\ldots\sigma_1\sigma_0\dual{\ell'}$ for some $p_1\in \eta_1$. 
%Thus there is some subset $\mathcal{I}\subseteq [1,n]$ such that $\sigma p_1 = \sigma_m'\ldots\sigma_1'\dual{\ell'}$ since FO-delete uses the same unifiers. 
Note that $p^\dagger = \sigma_p p = \sigma_p\sigma_n\ldots\sigma_1\sigma_0\dual{\ell'}$ (where the first equality holds since $p^\dagger$ corresponds to $p$, and thus the two literals are unifiable) but also that $\dual{\ell'} = \sigma_\ell\ell'$ for some $\sigma_\ell$ (by definition as $\ell$ is a pivot). So now we have $p^\dagger =  \sigma_p\sigma_n\ldots\sigma_1\sigma_0\sigma_\ell\ell'$, so letting $\sigma''=\sigma_p\sigma_m'\ldots\sigma_1'\sigma_\ell$ we have that $p^\dagger = \sigma'' \ell$, i.e. that $(p^\dagger,\ell^\dagger)$ are unifiable via $\sigma''$.

%Note that $p^\dagger =  \sigma_m'\ldots\sigma_1'\dual{\ell'}$ but also that $\dual{\ell'} = \sigma_\ell\ell'$ for some $\sigma_\ell$ (by definition as $\ell$ as a pivot). So now we have $p^\dagger =  \sigma_m'\ldots\sigma_1'\sigma''\ell$, so letting $\sigma''=\sigma_m'\ldots\sigma_1'\sigma_\ell$ we have that $p^\dagger = \sigma'' \ell$, i.e. that $(p^\dagger,\ell^\dagger)$ are unifiable via $\sigma''$, a contradiction.